Machines/Multiclock/TypedSoCTile.lean
@@ -1,0 +1,3 @@
+-- Copyright (c) 2026 Kevin Baragona
+-- SPDX-License-Identifier: Apache-2.0
+import Machines.Multiclock.TypedSoCTile.Design
